Language_Components/Seq/Seq.thy
@@ -51,13 +51,17 @@ definition seq_sem_lifting_schem1 where
 definition seq_sem_lifting_schem2 where
 "seq_sem_lifting_schem2 = (SP (SPRI (SO NC)) NX)"
 
+text_raw \<open>%Snippet gazelle__language_components__seq__seq_prio\<close>
 fun seq_prio :: "syn \<Rightarrow> nat" where
 "seq_prio _ = 2"
+text_raw \<open>%EndSnippet\<close>
 
+text_raw \<open>%Snippet gazelle__language_components__seq__seq_sem_lifting_gen\<close>
 definition seq_sem_lifting_gen :: "(syn, 'x state', ('x, 'a :: Pordb) control) lifting"
   where
 "seq_sem_lifting_gen = schem_lift
-    NC (SP (SPRC seq_prio (SO NC)) NX) "
+    NC (SP (SPRC seq_prio (SO NC)) NX)"
+text_raw \<open>%EndSnippet\<close>
 
 (* alternate definition that doesn't rely on auto lifter *)
 definition seq_sem_lifting' :: "(syn, 'x state', 'x state' md_triv option md_prio) lifting"
@@ -82,6 +86,7 @@ lemma seq_sem_lifting_gen_valid' :
   unfolding seq_sem_lifting'_def schem_lift_defs schem_lift_S_defs
   by(fastforce intro: lifting_valid_fast)
 
+text_raw \<open>%Snippet gazelle__language_components__seq__seq_sem_l_gen\<close>
 definition seq_sem_l_gen ::
   "('s \<Rightarrow> syn) \<Rightarrow>
    's \<Rightarrow> (('x, 'y :: Pordb) control) \<Rightarrow> (('x, 'y :: Pordb) control)" where
@@ -89,7 +94,7 @@ definition seq_sem_l_gen ::
   lift_map_s lfts
   seq_sem_lifting_gen
   seq_sem"
-
+text_raw \<open>%EndSnippet\<close>
 
 definition seq_semx :: 
 "('s \<Rightarrow> syn) \<Rightarrow>
